

Linear Differential Equations

- A first-order DE is said to be **linear** if it can be written in the (standard) form

$$\frac{dy}{dx} + P(x)y = Q(x) \quad (*)$$

- The characteristic feature of this equation is that it is linear in y and y' , whereas P and Q on the right may be any given functions of x .
- If the right side $Q(x)$ is **zero** for all x in the interval in which we consider the equation, the differential equation is said to be **homogeneous**; otherwise it is said to be **non-homogeneous**.

- Let us find a formula for the **general solution** of (*) in some interval I , assuming that P and Q are continuous in I .
- For the **homogeneous** equation

$$y' + P(x)y = 0$$

this is very simple. Indeed, by separating variables we have

$$\frac{dy}{y} = -P(x)dx, \text{ thus}$$

$$\ln |y| = -\int P(x)dx + C^*$$

and by taking exponents on both sides

$$y(x) = Ce^{-\int P(x)dx} \quad (C = \pm e^{C^*})$$

Here we may take $C = 0$ and obtain the **trivial solution** $y = 0$.

- The **non-homogeneous** equation (*) will now be solved. It turns out that it has the pleasant property of possessing an integrating factor depending only on x . That is,

$$I.F = e^{\int P dx}$$

- Now we multiply both sides of (*) by this I.F so that we get

$$\frac{dy}{dx} e^{\int P dx} + y e^{\int P dx} P(x) = Q(x) e^{\int P dx}$$
$$\Rightarrow \frac{d}{dx} \left(y e^{\int P dx} \right) = Q(x) e^{\int P dx}$$

- Finally integrate both sides of this last equation with respect to x , and then solve the resulting equation for y . i.e.

$$y e^{\int P dx} = \int Q(x) e^{\int P dx} dx + C$$

Example 1. Solve $y' - 3y = 6$.

Solution:

It is linear with $P(x) = -3$ and $Q(x) = 6$.

Here $\int P(x)dx = \int -3 dx = -3x$.

Thus $I(x) = e^{\int P(x)dx} = e^{-3x}$.

Multiplying the DE by the I.F, we obtain

$$e^{-3x}y' - 3e^{-3x}y = 6e^{-3x}$$

$$\text{or } \frac{d}{dx} (ye^{-3x}) = 6e^{-3x}$$

Integrating both sides with respect to x , we have

$$\int \frac{d}{dx} (ye^{-3x}) dx = \int 6e^{-3x} dx$$

$$ye^{-3x} = -2e^{-3x} + C$$

$$y = Ce^{3x} - 2. \quad \square$$

Note: No need to include the constant of integration while calculating I.F.

Example 2. Find an integrating factor and then solve the DE $\frac{dy}{dx} - 2xy = x$.

Solution: The DE is linear with $P(x) = -2x$

and $Q(x) = x$. Hence

$$I(x) = e^{\int P(x)dx} = e^{\int (-2x)dx} = e^{-x^2}.$$

Now multiplying the DE by this $I(x)$, we get

$$e^{-x^2} y' - 2xe^{-x^2} y = x e^{-x^2}$$

$$\frac{d}{dx} (ye^{-x^2}) = x e^{-x^2}$$

Integrating both sides, we have

$$\int \frac{d}{dx} (ye^{-x^2}) dx = \int x e^{-x^2} dx$$

$$ye^{-x^2} = -\frac{1}{2}e^{-x^2} + C \quad \text{or} \quad y = Ce^{x^2} - \frac{1}{2}. \quad \square$$

Exercises

1. Solve $y' + y = \sin x$.

Ans. $y = Ce^{-x} + \frac{1}{2} \sin x - \frac{1}{2} \cos x$

2. Solve $\frac{dz}{dx} - xz = -x$.

Ans. $z(x) = Ce^{\frac{x^2}{2}} + 1$.

3. Solve the IVP $y' + y \tan x = \sin 2x$, $y(0) = 1$.

Ans. $y(x) = C \cos x - 2 \cos^2 x$,

and using the initial condition, we get $C = 3$.

Therefore, $y = 3 \cos x - 2 \cos^2 x$.

Bernoulli's Equation

(Reduction to Linear form)

- It is named after the Swiss mathematician *Jakob Bernoulli* who is known for his basic work in probability and elasticity theory.
- Certain nonlinear DEs can be reduced to linear form. The practically most famous of these is the Bernoulli equation. It has the form

$$\frac{dy}{dx} + P(x)y = Q(x)y^n \quad (**)$$

where n is a real number.

If $n = 0$ or $n = 1$, the equation is **linear**.

- To solve (**), divide both sides by y^n , so that

$$y^{-n} \frac{dy}{dx} + P(x)y^{1-n} = Q(x) \quad (* * *)$$

Put $y^{1-n} = z$ so that $(1-n)y^{-n} \frac{dy}{dx} = \frac{dz}{dx}$.

Thus $(* * *)$ becomes

$$\frac{1}{1-n} \frac{dz}{dx} + P(x)z = Q(x) \quad \text{or}$$

$$\frac{dz}{dx} + (1-n)P(x)z = (1-n)Q(x)$$

which is **linear** in z .

Example 1. Solve $y' + xy = xy^2$.

Solution: This equation is not linear. It is, however, a Bernoulli DE with $P(x) = Q(x) = x$, and $n = 2$. We now make the substitution $z = y^{1-n} = y^{-1}$, from which follow

$$y = \frac{1}{z} \quad \text{and} \quad y' = -\frac{1}{z^2}z'$$

Substituting these equations into the DE, we get

$$-\frac{z'}{z^2} + \frac{x}{z} = \frac{x}{z^2}$$

$$\Rightarrow z' - xz = -x, \quad \text{which is linear.}$$

Its solution is $z = Ce^{\frac{x^2}{2}} + 1$. (Show!)

The solution of the original DE is then

$$y = \frac{1}{z} = \frac{1}{Ce^{\frac{x^2}{2}} + 1}. \quad \square$$

Example 2. Solve $y' - \frac{3}{x}y = x^4 y^{\frac{1}{3}}$.

Solution: This is a Bernoulli DE with $P(x) = -\frac{3}{x}$, $Q(x) = x^4$, and $n = 1/3$. Using the substitution $z = y^{1-n} = y^{1-\frac{1}{3}} = y^{\frac{2}{3}}$, we have

$$y = z^{\frac{3}{2}} \quad \text{and} \quad y' = \frac{3}{2}z^{\frac{1}{2}}z'.$$

Substituting these values into the DE, we get

$$\frac{3}{2}z^{\frac{1}{2}}z' - \frac{3}{x}z^{\frac{3}{2}} = x^4z^{\frac{1}{2}}$$

$$\text{or } z' - \frac{2}{x}z = \frac{2}{3}x^4, \text{ which is linear.}$$

Its solution is $z = Cx^2 + \frac{2}{9}x^5$.

Since $z = y^{\frac{2}{3}}$, the solution of the original problem is given implicitly by

$$y^{\frac{2}{3}} = Cx^2 + \frac{2}{9}x^5. \quad \square$$

Exercise

1. Solve $x \frac{dy}{dx} + y = x^3 y^6$.

Ans. $1 = (\frac{5}{2} + Cx^2)x^3 y^5$.

2. Solve the DE $(x + 3y + 2) \frac{dy}{dx} = 1$.

Ans. It is not linear in y and $\frac{dy}{dx}$.

But writing it in the form $\frac{dx}{dy} = x + 3y + 2$

or $\frac{dx}{dy} - x = 3y + 2$, it is linear in x and $\frac{dx}{dy}$.

Its solution is $x = -3y - 5 + Ce^y$.